Ski.lean
@@ -5,3 +5,9 @@ import Ski.Basic
 import Ski.Combinator
 import Ski.Quote
 import Ski.Rice
+import Ski.Model
+import Ski.Register
+import Ski.RegisterEncode
+import Ski.Simulation
+import Ski.SkiModel
+import Ski.RegisterModel
